TODO: Prove coherence implies Lmatch

2016/Ext_Structures.thy
@@ -99,7 +99,7 @@ inductive eval1_L :: "lterm \<Rightarrow> lterm \<Rightarrow> bool" where
   eval1_L_ProjR:
     "eval1_L t1 t1' \<Longrightarrow> eval1_L (ProjR i t1) (ProjR i t1')" |
   eval1_L_RCD:
-    " l\<in>set L \<Longrightarrow> index L l = m \<Longrightarrow> is_value_L (Record (take m L) (take m LT)) \<Longrightarrow> 
+    " m<length LT \<Longrightarrow> is_value_L (Record (take m L) (take m LT)) \<Longrightarrow> 
       eval1_L (LT ! m) (t') \<Longrightarrow> eval1_L (Record L LT) (Record L (replace m t' LT))" |   
  -- "Rules relating to evaluation of pattern matching"
   eval1_L_LetPV:
@@ -161,161 +161,174 @@ text{*  For the typing rule of letbinder, we require to replace the type
     *}
 
 
-inductive has_type_L :: "lcontext \<Rightarrow> lterm \<Rightarrow> pcontext \<Rightarrow> ltype \<Rightarrow> bool" ("((_)/ \<turnstile> \<lparr>(_)|;|(_)\<rparr>/ |:| (_))" [150, 150, 150, 150] 150) where
+inductive has_type_L :: "lcontext \<Rightarrow> lterm \<Rightarrow> pcontext \<Rightarrow> bool \<Rightarrow> ltype \<Rightarrow> bool" ("((_)/ \<turnstile> \<lparr>(_)|;|(_),(_)\<rparr>/ |:| (_))" [150, 150, 150, 150,150] 150) where
   -- "Rules relating to the type of Booleans"
   has_type_LTrue:
-    "\<Gamma> \<turnstile> \<lparr>LTrue|;| \<sigma>\<rparr> |:| Bool" |
+    "\<Gamma> \<turnstile> \<lparr>LTrue|;| \<sigma>, f\<rparr> |:| Bool" |
   has_type_LFalse:
-    "\<Gamma> \<turnstile> \<lparr>LFalse|;| \<sigma>\<rparr> |:| Bool" |
+    "\<Gamma> \<turnstile> \<lparr>LFalse|;| \<sigma>, f\<rparr> |:| Bool" |
   has_type_LIf:
-    "\<Gamma> \<turnstile> \<lparr>t1|;| \<sigma>\<rparr> |:| Bool \<Longrightarrow> \<Gamma> \<turnstile> \<lparr>t2|;| \<sigma>\<rparr> |:| T' \<Longrightarrow> \<Gamma> \<turnstile> \<lparr>t3|;| \<sigma>\<rparr> |:| T' \<Longrightarrow> 
-      \<Gamma> \<turnstile> \<lparr>LIf t1 t2 t3|;| \<sigma>\<rparr> |:| T'" |
+    "\<Gamma> \<turnstile> \<lparr>t1|;| \<sigma>,f\<rparr> |:| Bool \<Longrightarrow> \<Gamma> \<turnstile> \<lparr>t2|;| \<sigma>,f\<rparr> |:| T' \<Longrightarrow> \<Gamma> \<turnstile> \<lparr>t3|;| \<sigma>,f\<rparr> |:| T' \<Longrightarrow> 
+      \<Gamma> \<turnstile> \<lparr>LIf t1 t2 t3|;| \<sigma>,f\<rparr> |:| T'" |
 
   -- \<open>Rules relating to the type of the constructs of the $\lambda$-calculus\<close>
   has_type_LVar:
-    "(x, T') |\<in>| \<Gamma> \<Longrightarrow> \<Gamma> \<turnstile> \<lparr>LVar x|;| \<sigma>\<rparr> |:| (T')" |
+    "(x, T') |\<in>| \<Gamma> \<Longrightarrow> \<Gamma> \<turnstile> \<lparr>LVar x|;| \<sigma>,f\<rparr> |:| (T')" |
   has_type_LAbs:
-    "(\<Gamma> |,| T1) \<turnstile> \<lparr>t2|;| \<sigma>\<rparr> |:| T2 \<Longrightarrow> \<Gamma> \<turnstile> \<lparr>LAbs T1 t2|;| \<sigma>\<rparr> |:| (T1 \<rightarrow> T2)" |
+    "(\<Gamma> |,| T1) \<turnstile> \<lparr>t2|;| \<sigma>,f\<rparr> |:| T2 \<Longrightarrow> \<Gamma> \<turnstile> \<lparr>LAbs T1 t2|;| \<sigma>,f\<rparr> |:| (T1 \<rightarrow> T2)" |
   has_type_LApp:
-    "\<Gamma> \<turnstile> \<lparr>t1|;| \<sigma>\<rparr> |:| (T11 \<rightarrow> T12) \<Longrightarrow> \<Gamma> \<turnstile> \<lparr>t2|;| \<sigma>\<rparr> |:| T11 \<Longrightarrow> 
-      \<Gamma> \<turnstile> \<lparr>LApp t1 t2|;| \<sigma>\<rparr> |:| T12" |  
+    "\<Gamma> \<turnstile> \<lparr>t1|;| \<sigma>,f\<rparr> |:| (T11 \<rightarrow> T12) \<Longrightarrow> \<Gamma> \<turnstile> \<lparr>t2|;| \<sigma>,f\<rparr> |:| T11 \<Longrightarrow> 
+      \<Gamma> \<turnstile> \<lparr>LApp t1 t2|;| \<sigma>,f\<rparr> |:| T12" |  
   has_type_LUnit:
-    "\<Gamma> \<turnstile> \<lparr>unit|;| \<sigma>\<rparr> |:| Unit " |  
+    "\<Gamma> \<turnstile> \<lparr>unit|;| \<sigma>,f\<rparr> |:| Unit " |  
   has_type_LSeq:
-    "\<Gamma> \<turnstile> \<lparr>t1|;| \<sigma>\<rparr> |:| Unit \<Longrightarrow> \<Gamma> \<turnstile> \<lparr>t2|;| \<sigma>\<rparr> |:| A \<Longrightarrow> \<Gamma> \<turnstile> \<lparr>Seq t1 t2|;| \<sigma>\<rparr> |:| A" |
+    "\<Gamma> \<turnstile> \<lparr>t1|;| \<sigma>,f\<rparr> |:| Unit \<Longrightarrow> \<Gamma> \<turnstile> \<lparr>t2|;| \<sigma>,f\<rparr> |:| A \<Longrightarrow> \<Gamma> \<turnstile> \<lparr>Seq t1 t2|;| \<sigma>,f\<rparr> |:| A" |
   has_type_LAscribe:
-    "\<Gamma> \<turnstile> \<lparr>t1|;| \<sigma>\<rparr> |:| A \<Longrightarrow> \<Gamma> \<turnstile> \<lparr>t1 as A|;| \<sigma>\<rparr> |:| A" |
+    "\<Gamma> \<turnstile> \<lparr>t1|;| \<sigma>,f\<rparr> |:| A \<Longrightarrow> \<Gamma> \<turnstile> \<lparr>t1 as A|;| \<sigma>,f\<rparr> |:| A" |
   has_type_Let:
-    "\<Gamma> \<turnstile> \<lparr>t1|;| \<sigma>\<rparr> |:| A \<Longrightarrow> (insert_nth x A \<Gamma>) \<turnstile> \<lparr> t2|;| \<sigma>\<rparr> |:| B \<Longrightarrow> 
-      \<Gamma> \<turnstile> \<lparr>Let var x := t1 in t2|;| \<sigma>\<rparr> |:| B" |
+    "\<Gamma> \<turnstile> \<lparr>t1|;| \<sigma>,f\<rparr> |:| A \<Longrightarrow> (insert_nth x A \<Gamma>) \<turnstile> \<lparr> t2|;| \<sigma>,f\<rparr> |:| B \<Longrightarrow> 
+      \<Gamma> \<turnstile> \<lparr>Let var x := t1 in t2|;| \<sigma>,f\<rparr> |:| B" |
   has_type_Pair:
-    "\<Gamma> \<turnstile> \<lparr>t1|;| \<sigma>\<rparr> |:| A \<Longrightarrow> \<Gamma> \<turnstile> \<lparr>t2|;| \<sigma>\<rparr> |:| B \<Longrightarrow> 
-      \<Gamma> \<turnstile> \<lparr>\<lbrace>t1,t2\<rbrace>|;| \<sigma>\<rparr> |:| A |\<times>| B" |
+    "\<Gamma> \<turnstile> \<lparr>t1|;| \<sigma>,f\<rparr> |:| A \<Longrightarrow> \<Gamma> \<turnstile> \<lparr>t2|;| \<sigma>,f\<rparr> |:| B \<Longrightarrow> 
+      \<Gamma> \<turnstile> \<lparr>\<lbrace>t1,t2\<rbrace>|;| \<sigma>,f\<rparr> |:| A |\<times>| B" |
   has_type_Proj1:
-    "\<Gamma> \<turnstile> \<lparr>t1|;| \<sigma>\<rparr> |:| A |\<times>| B \<Longrightarrow> \<Gamma> \<turnstile> \<lparr>\<pi>1 t1|;| \<sigma>\<rparr> |:| A" |
+    "\<Gamma> \<turnstile> \<lparr>t1|;| \<sigma>,f\<rparr> |:| A |\<times>| B \<Longrightarrow> \<Gamma> \<turnstile> \<lparr>\<pi>1 t1|;| \<sigma>,f\<rparr> |:| A" |
   has_type_Proj2:
-    "\<Gamma> \<turnstile> \<lparr>t1|;| \<sigma>\<rparr> |:| A |\<times>| B \<Longrightarrow> \<Gamma> \<turnstile> \<lparr>\<pi>2 t1|;| \<sigma>\<rparr> |:| B" |
+    "\<Gamma> \<turnstile> \<lparr>t1|;| \<sigma>,f\<rparr> |:| A |\<times>| B \<Longrightarrow> \<Gamma> \<turnstile> \<lparr>\<pi>2 t1|;| \<sigma>,f\<rparr> |:| B" |
   has_type_Tuple:
     "L\<noteq>[] \<Longrightarrow> length L = length TL \<Longrightarrow> 
-      (\<And>i. 0\<le>i \<Longrightarrow> i< length L \<Longrightarrow> \<Gamma> \<turnstile> \<lparr>(L ! i)|;| \<sigma>\<rparr> |:| (TL ! i))
-      \<Longrightarrow> \<Gamma> \<turnstile> \<lparr>Tuple L|;| \<sigma>\<rparr> |:| \<lparr>TL\<rparr>" |
+      (\<And>i. 0\<le>i \<Longrightarrow> i< length L \<Longrightarrow> \<Gamma> \<turnstile> \<lparr>(L ! i)|;| \<sigma>,f\<rparr> |:| (TL ! i))
+      \<Longrightarrow> \<Gamma> \<turnstile> \<lparr>Tuple L|;| \<sigma>,f\<rparr> |:| \<lparr>TL\<rparr>" |
   has_type_ProjT:
-    "1\<le>i \<Longrightarrow> i\<le> length TL \<Longrightarrow> \<Gamma> \<turnstile> \<lparr>t|;| \<sigma>\<rparr> |:| \<lparr>TL\<rparr> \<Longrightarrow> 
-      \<Gamma> \<turnstile> \<lparr>\<Pi> i t|;| \<sigma>\<rparr> |:| (TL ! (i-1))" |
+    "1\<le>i \<Longrightarrow> i\<le> length TL \<Longrightarrow> \<Gamma> \<turnstile> \<lparr>t|;| \<sigma>,f\<rparr> |:| \<lparr>TL\<rparr> \<Longrightarrow> 
+      \<Gamma> \<turnstile> \<lparr>\<Pi> i t|;| \<sigma>,f\<rparr> |:| (TL ! (i-1))" |
   has_type_RCD:
     "L\<noteq>[] \<Longrightarrow> distinct L \<Longrightarrow> length LT = length TL \<Longrightarrow> length L = length LT \<Longrightarrow>
-      (\<And>i. i< length LT \<Longrightarrow> \<Gamma> \<turnstile> \<lparr>(LT ! i)|;| \<sigma>\<rparr> |:| (TL ! i))
-      \<Longrightarrow> \<Gamma> \<turnstile> \<lparr>Record L LT|;| \<sigma>\<rparr> |:| \<lparr>L|:|TL\<rparr>" |
+      (\<And>i. i< length LT \<Longrightarrow> \<Gamma> \<turnstile> \<lparr>(LT ! i)|;| \<sigma>,f\<rparr> |:| (TL ! i))
+      \<Longrightarrow> \<Gamma> \<turnstile> \<lparr>Record L LT|;| \<sigma>,f\<rparr> |:| \<lparr>L|:|TL\<rparr>" |
   has_type_ProjR:
     "distinct L1 \<Longrightarrow> l\<in> set L1  \<Longrightarrow> length L1 = length TL \<Longrightarrow> 
-      \<Gamma> \<turnstile> \<lparr>t|;| \<sigma>\<rparr> |:| \<lparr>L1|:|TL\<rparr> \<Longrightarrow> 
-      \<Gamma> \<turnstile> \<lparr>ProjR l t|;| \<sigma>\<rparr> |:| (TL ! index L1 l)" |
+      \<Gamma> \<turnstile> \<lparr>t|;| \<sigma>,f\<rparr> |:| \<lparr>L1|:|TL\<rparr> \<Longrightarrow> 
+      \<Gamma> \<turnstile> \<lparr>ProjR l t|;| \<sigma>,f\<rparr> |:| (TL ! index L1 l)" |
   has_type_PatternVar:
-    "\<sigma> k = Some A \<Longrightarrow> \<Gamma> \<turnstile> \<lparr><|V k as A|>|;| \<sigma>\<rparr> |:| A" |
+    "\<sigma> k = Some A \<Longrightarrow> \<Gamma> \<turnstile> \<lparr><|V k as A|>|;| \<sigma>,f\<rparr> |:| A" |
   has_type_LetPattern:
-    "coherent p B\<Longrightarrow> Lmatch_Type p \<sigma> \<Longrightarrow> \<Gamma> \<turnstile> \<lparr>t1|;| \<sigma>1\<rparr> |:| B \<Longrightarrow>
-     \<Gamma> \<turnstile> \<lparr>t2|;|(\<sigma> ++ \<sigma>1)\<rparr> |:| A \<Longrightarrow> \<Gamma> \<turnstile> \<lparr>Let pattern p := t1 in t2|;| \<sigma>1\<rparr> |:| A" |
+    "coherent p B\<Longrightarrow> Lmatch_Type p \<sigma> \<Longrightarrow> \<Gamma> \<turnstile> \<lparr>t1|;| \<sigma>1,f\<rparr> |:| B \<Longrightarrow>
+     \<Gamma> \<turnstile> \<lparr>t2|;|(\<sigma> ++ \<sigma>1), f\<rparr> |:| A \<Longrightarrow> \<Gamma> \<turnstile> \<lparr>Let pattern p := t1 in t2|;| \<sigma>1, f\<rparr> |:| A" |
   has_type_Inl:
-    "\<Gamma> \<turnstile> \<lparr>t1|;| \<sigma>1\<rparr> |:| A \<Longrightarrow> \<Gamma> \<turnstile> \<lparr>inl t1 as A|+|B |;|\<sigma>1\<rparr> |:| A|+|B" |
+    "\<Gamma> \<turnstile> \<lparr>t1|;| \<sigma>1,f\<rparr> |:| A \<Longrightarrow> \<Gamma> \<turnstile> \<lparr>inl t1 as A|+|B |;|\<sigma>1,f\<rparr> |:| A|+|B" |
   has_type_Inr:
-    "\<Gamma> \<turnstile> \<lparr>t1|;| \<sigma>1\<rparr> |:| B \<Longrightarrow> \<Gamma> \<turnstile> \<lparr>inr t1 as A|+|B |;| \<sigma>1\<rparr> |:| A|+|B" |
+    "\<Gamma> \<turnstile> \<lparr>t1|;| \<sigma>1,f\<rparr> |:| B \<Longrightarrow> \<Gamma> \<turnstile> \<lparr>inr t1 as A|+|B |;| \<sigma>1,f\<rparr> |:| A|+|B" |
   has_type_Case:
-    "\<Gamma> \<turnstile> \<lparr> t|;| \<sigma>1 \<rparr> |:| A|+|B \<Longrightarrow> insert_nth x A \<Gamma> \<turnstile> \<lparr>t1|;| \<sigma>1\<rparr> |:| C \<Longrightarrow>
-     insert_nth y B \<Gamma> \<turnstile> \<lparr>t2|;| \<sigma>1\<rparr> |:| C \<Longrightarrow> 
-     \<Gamma> \<turnstile> \<lparr>Case t of Inl x \<Rightarrow> t1 | Inr y \<Rightarrow> t2 |;| \<sigma>1\<rparr> |:| C" |
+    "\<Gamma> \<turnstile> \<lparr> t|;| \<sigma>1,f \<rparr> |:| A|+|B \<Longrightarrow> insert_nth x A \<Gamma> \<turnstile> \<lparr>t1|;| \<sigma>1,f\<rparr> |:| C \<Longrightarrow>
+     insert_nth y B \<Gamma> \<turnstile> \<lparr>t2|;| \<sigma>1,f\<rparr> |:| C \<Longrightarrow> 
+     \<Gamma> \<turnstile> \<lparr>Case t of Inl x \<Rightarrow> t1 | Inr y \<Rightarrow> t2 |;| \<sigma>1,f\<rparr> |:| C" |
   has_type_Variant:
-    "\<Gamma> \<turnstile> \<lparr> t |;| \<sigma> \<rparr> |:| (TL!i) \<Longrightarrow> 
-      \<Gamma> \<turnstile> \<lparr> <(L!i):=t> as <L|,|TL> |;|\<sigma> \<rparr> |:| <L|,|TL>" |
+    "i<length L \<Longrightarrow> length L=length TL \<Longrightarrow> \<Gamma> \<turnstile> \<lparr> t |;| \<sigma>,f \<rparr> |:| (TL!i) \<Longrightarrow> 
+      \<Gamma> \<turnstile> \<lparr> <(L!i):=t> as <L|,|TL> |;|\<sigma>,f \<rparr> |:| <L|,|TL>" |
   has_type_CaseV:
     " L\<noteq>\<emptyset> \<Longrightarrow> length I = length L \<Longrightarrow> length L = length TL \<Longrightarrow> 
       length L = length LT \<Longrightarrow>
-      \<Gamma> \<turnstile> \<lparr> t |;| \<sigma> \<rparr> |:| <L|,|TL> \<Longrightarrow> 
-      (\<forall>i<length L. insert_nth (I!i) (TL!i) \<Gamma> \<turnstile> \<lparr>(LT!i)|;| \<sigma>\<rparr> |:| A) \<Longrightarrow>
-      \<Gamma> \<turnstile> \<lparr> Case t of <L:=I> \<Rightarrow> LT |;| \<sigma>\<rparr> |:| A" |
+      \<Gamma> \<turnstile> \<lparr> t |;| \<sigma>,f \<rparr> |:| <L|,|TL> \<Longrightarrow> 
+      (\<forall>i<length L. insert_nth (I!i) (TL!i) \<Gamma> \<turnstile> \<lparr>(LT!i)|;| \<sigma>,f\<rparr> |:| A) \<Longrightarrow>
+      \<Gamma> \<turnstile> \<lparr> Case t of <L:=I> \<Rightarrow> LT |;| \<sigma>,f\<rparr> |:| A" |
   has_type_Fix:
-    "\<Gamma> \<turnstile> \<lparr> t |;| \<sigma>\<rparr> |:| A\<rightarrow>A \<Longrightarrow> \<Gamma> \<turnstile> \<lparr> fix t |;| \<sigma>\<rparr> |:| A"|
+    "\<Gamma> \<turnstile> \<lparr> t |;| \<sigma>,f\<rparr> |:| A\<rightarrow>A \<Longrightarrow> \<Gamma> \<turnstile> \<lparr> fix t |;| \<sigma>,f\<rparr> |:| A"|
   has_type_Nil:
-    "\<Gamma> \<turnstile> \<lparr> Lnil A |;| \<sigma>\<rparr> |:| \<lambda>List A"|
+    "\<Gamma> \<turnstile> \<lparr> Lnil A |;| \<sigma>, False\<rparr> |:| \<lambda>List A"|
   has_type_isNil:
-    "\<Gamma> \<turnstile> \<lparr> t|;| \<sigma> \<rparr> |:| \<lambda>List A \<Longrightarrow>\<Gamma> \<turnstile> \<lparr> Lisnil A t|;| \<sigma> \<rparr> |:| Bool"| 
+    "\<Gamma> \<turnstile> \<lparr> t|;| \<sigma>,f \<rparr> |:| \<lambda>List A \<Longrightarrow>\<Gamma> \<turnstile> \<lparr> Lisnil A t|;| \<sigma>,f \<rparr> |:| Bool"| 
   has_type_head:
-    "\<Gamma> \<turnstile> \<lparr> t|;| \<sigma> \<rparr> |:| \<lambda>List A \<Longrightarrow>\<Gamma> \<turnstile> \<lparr> Lhead A t|;| \<sigma> \<rparr> |:| A"| 
+    "\<Gamma> \<turnstile> \<lparr> t|;| \<sigma>,True \<rparr> |:| \<lambda>List A \<Longrightarrow>\<Gamma> \<turnstile> \<lparr> Lhead A t|;| \<sigma>,f \<rparr> |:| A"| 
   has_type_tail:
-    "\<Gamma> \<turnstile> \<lparr> t|;| \<sigma> \<rparr> |:| \<lambda>List A \<Longrightarrow>\<Gamma> \<turnstile> \<lparr> Ltail A t|;| \<sigma> \<rparr> |:| A"| 
+    "\<Gamma> \<turnstile> \<lparr> t|;| \<sigma>,True \<rparr> |:| \<lambda>List A \<Longrightarrow>\<Gamma> \<turnstile> \<lparr> Ltail A t|;| \<sigma>,f \<rparr> |:| \<lambda>List A"| 
   has_type_cons:
-    "\<Gamma> \<turnstile> \<lparr> t|;| \<sigma> \<rparr> |:| A \<Longrightarrow> \<Gamma> \<turnstile> \<lparr> t' |;| \<sigma> \<rparr> |:| A \<Longrightarrow>
-      \<Gamma> \<turnstile> \<lparr> Lcons A t t'|;| \<sigma> \<rparr> |:| \<lambda>List A"  
+    "\<Gamma> \<turnstile> \<lparr> t|;| \<sigma>,f \<rparr> |:| A \<Longrightarrow> \<Gamma> \<turnstile> \<lparr> t' |;| \<sigma>,f \<rparr> |:| \<lambda>List A \<Longrightarrow>
+      \<Gamma> \<turnstile> \<lparr> Lcons A t t'|;| \<sigma>,f \<rparr> |:| \<lambda>List A"  
 
-inductive_cases has_type_LetE : "\<Gamma> \<turnstile> \<lparr> Let var x := t1 in t2|;|\<sigma>1\<rparr>  |:| B"
-inductive_cases has_type_ProjTE: "\<Gamma> \<turnstile> \<lparr> \<Pi> i t|;|\<sigma>1\<rparr> |:| R"
-inductive_cases has_type_ProjRE: "\<Gamma> \<turnstile> \<lparr> ProjR l t|;|\<sigma>1\<rparr> |:| R"
-inductive_cases has_type_LetPE: "\<Gamma> \<turnstile> \<lparr>Let pattern p := t1 in t2|;|\<sigma>1\<rparr> |:| A"
-inductive_cases has_type_CaseSE: "\<Gamma> \<turnstile> \<lparr>Case t of Inl x \<Rightarrow> t1 | Inr y \<Rightarrow> t2|;|\<sigma>1\<rparr> |:| R"
-inductive_cases has_type_CaseVE: "\<Gamma> \<turnstile> \<lparr>Case t of <L:=I> \<Rightarrow> LT|;|\<sigma>1\<rparr> |:| R"
-inductive_cases has_type_LAbsE: "\<Gamma> \<turnstile> \<lparr>LAbs T1 t2|;|\<sigma>1\<rparr> |:| R"
-inductive_cases has_type_VariantE: "\<Gamma> \<turnstile> \<lparr><l:=t> as R |;|\<sigma>1\<rparr> |:| R"
+inductive_cases has_type_LetE : "\<Gamma> \<turnstile> \<lparr> Let var x := t1 in t2|;|\<sigma>,f\<rparr>  |:| B"
+inductive_cases has_type_ProjTE: "\<Gamma> \<turnstile> \<lparr> \<Pi> i t|;|\<sigma>1,f\<rparr> |:| R"
+inductive_cases has_type_ProjRE: "\<Gamma> \<turnstile> \<lparr> ProjR l t|;|\<sigma>1,f\<rparr> |:| R"
+inductive_cases has_type_LetPE: "\<Gamma> \<turnstile> \<lparr>Let pattern p := t1 in t2|;|\<sigma>1,f\<rparr> |:| A"
+inductive_cases has_type_CaseSE: "\<Gamma> \<turnstile> \<lparr>Case t of Inl x \<Rightarrow> t1 | Inr y \<Rightarrow> t2|;|\<sigma>1,f\<rparr> |:| R"
+inductive_cases has_type_CaseVE: "\<Gamma> \<turnstile> \<lparr>Case t of <L:=I> \<Rightarrow> LT|;|\<sigma>1,f\<rparr> |:| R"
+inductive_cases has_type_LAbsE: "\<Gamma> \<turnstile> \<lparr>LAbs T1 t2|;|\<sigma>1,f\<rparr> |:| R"
+inductive_cases has_type_VariantE: "\<Gamma> \<turnstile> \<lparr><l:=t> as R1 |;|\<sigma>1,f\<rparr> |:| R"
 
 lemma record_patterns_characterisation:
   "set (patterns (<|RCD L PL|>)) \<subseteq> S \<Longrightarrow> x \<in> set PL \<Longrightarrow> set(patterns (<|x|>)) \<subseteq> S"
 by (induction PL arbitrary: S x, auto) 
 
 lemma inversion:
-  "\<Gamma> \<turnstile> \<lparr> LTrue |;| \<sigma>\<rparr> |:| R \<Longrightarrow> R = Bool"
-  "\<Gamma> \<turnstile> \<lparr> LFalse |;| \<sigma>\<rparr> |:| R \<Longrightarrow> R = Bool"
-  "\<Gamma> \<turnstile> \<lparr> LIf t1 t2 t3 |;| \<sigma>\<rparr> |:| R \<Longrightarrow>  \<Gamma> \<turnstile> \<lparr>t1|;| \<sigma>\<rparr> |:| Bool \<and> \<Gamma> \<turnstile> \<lparr>t2|;| \<sigma>\<rparr> |:| R \<and> \<Gamma> \<turnstile> \<lparr>t3|;| \<sigma>\<rparr> |:| R"
-  "\<Gamma> \<turnstile> \<lparr> LVar x|;| \<sigma>\<rparr> |:| R \<Longrightarrow> (x, R) |\<in>| \<Gamma>"
-  "\<Gamma> \<turnstile> \<lparr> LAbs T1 t2 |;| \<sigma>\<rparr> |:| R \<Longrightarrow> \<exists>R2. R = T1 \<rightarrow> R2 \<and>  \<Gamma> |,| T1 \<turnstile> \<lparr>t2|;| \<sigma>\<rparr> |:| R2 "
-  "\<Gamma> \<turnstile> \<lparr> LApp t1 t2 |;| \<sigma>\<rparr> |:| R \<Longrightarrow> \<exists>T11. \<Gamma> \<turnstile> \<lparr>t1|;| \<sigma>\<rparr> |:| T11 \<rightarrow> R \<and> \<Gamma> \<turnstile> \<lparr>t2|;| \<sigma>\<rparr> |:| T11"
-  "\<Gamma> \<turnstile> \<lparr> unit|;| \<sigma>\<rparr> |:| R \<Longrightarrow> R = Unit"
-  "\<Gamma> \<turnstile> \<lparr> Seq t1 t2 |;| \<sigma>\<rparr> |:| R \<Longrightarrow> \<exists>A. R = A \<and> \<Gamma> \<turnstile> \<lparr>t2|;| \<sigma>\<rparr> |:| A \<and> \<Gamma> \<turnstile> \<lparr>t1|;| \<sigma>\<rparr> |:| Unit"
-  "\<Gamma> \<turnstile> \<lparr> t as A |;| \<sigma>\<rparr> |:| R \<Longrightarrow> R = A"
-  "\<Gamma> \<turnstile> \<lparr> Let var x := t in t1 |;| \<sigma>\<rparr> |:| R \<Longrightarrow> \<exists>A B. R = B \<and> \<Gamma> \<turnstile> \<lparr> t|;| \<sigma>\<rparr> |:| A \<and> (insert_nth x A \<Gamma>) \<turnstile> \<lparr>t1|;| \<sigma>\<rparr> |:| B"
-  "\<Gamma> \<turnstile> \<lparr> \<lbrace>t1,t2\<rbrace>|;| \<sigma>\<rparr> |:| R \<Longrightarrow> \<exists>A B. \<Gamma> \<turnstile> \<lparr> t1|;| \<sigma>\<rparr> |:| A \<and> \<Gamma> \<turnstile> \<lparr> t2|;| \<sigma>\<rparr> |:| B \<and> R = A |\<times>| B"
-  "\<Gamma> \<turnstile> \<lparr> \<pi>1 t|;| \<sigma>\<rparr> |:| R \<Longrightarrow> \<exists>A B. \<Gamma> \<turnstile> \<lparr> t|;| \<sigma>\<rparr> |:| A |\<times>| B \<and> R = A"
-  "\<Gamma> \<turnstile> \<lparr> \<pi>2 t|;| \<sigma>\<rparr> |:| R \<Longrightarrow> \<exists>A B. \<Gamma> \<turnstile> \<lparr> t|;| \<sigma>\<rparr> |:| A |\<times>| B \<and> R = B"
-  "\<Gamma> \<turnstile> \<lparr> Tuple L|;| \<sigma>\<rparr> |:| R \<Longrightarrow> \<exists>TL. length L = length TL \<and> (\<forall>i. 0\<le>i \<longrightarrow> i< length L \<longrightarrow> \<Gamma> \<turnstile> \<lparr>(L ! i)|;| \<sigma>\<rparr> |:| (TL ! i)) \<and> R = \<lparr>TL\<rparr>"
-  "\<Gamma> \<turnstile> \<lparr> (\<Pi> i t)|;| \<sigma>\<rparr> |:| R \<Longrightarrow> \<exists>TL. R = (TL ! (i-1)) \<and> \<Gamma> \<turnstile> \<lparr>t|;| \<sigma>\<rparr> |:| \<lparr>TL\<rparr> \<and> 1\<le>i \<and> i\<le> length TL"
-  "\<Gamma> \<turnstile> \<lparr> (Record L1 LT)|;| \<sigma>\<rparr> |:| R \<Longrightarrow> \<exists>TL. R = \<lparr>L1|:|TL\<rparr> \<and> length TL = length LT \<and> length L1 = length LT \<and> distinct L1 \<and> 
-                                    (\<forall>i. 0\<le>i \<longrightarrow> i< length LT \<longrightarrow> \<Gamma> \<turnstile> \<lparr> (LT ! i)|;| \<sigma>\<rparr> |:| (TL ! i)) " 
-  "\<Gamma> \<turnstile> \<lparr> (ProjR l t)|;| \<sigma>\<rparr> |:| R \<Longrightarrow>\<exists>m L TL. \<Gamma> \<turnstile> \<lparr>t |;| \<sigma>\<rparr> |:| \<lparr>L|:|TL\<rparr> \<and> index L l = m \<and> TL ! m = R \<and> distinct L \<and> length L = length TL
+  "\<Gamma> \<turnstile> \<lparr> LTrue |;| \<sigma>,f\<rparr> |:| R \<Longrightarrow> R = Bool"
+  "\<Gamma> \<turnstile> \<lparr> LFalse |;| \<sigma>,f\<rparr> |:| R \<Longrightarrow> R = Bool"
+  "\<Gamma> \<turnstile> \<lparr> LIf t1 t2 t3 |;| \<sigma>,f\<rparr> |:| R \<Longrightarrow>  \<Gamma> \<turnstile> \<lparr>t1|;| \<sigma>,f\<rparr> |:| Bool \<and> \<Gamma> \<turnstile> \<lparr>t2|;| \<sigma>,f\<rparr> |:| R \<and> \<Gamma> \<turnstile> \<lparr>t3|;| \<sigma>,f\<rparr> |:| R"
+  "\<Gamma> \<turnstile> \<lparr> LVar x|;| \<sigma>,f\<rparr> |:| R \<Longrightarrow> (x, R) |\<in>| \<Gamma>"
+  "\<Gamma> \<turnstile> \<lparr> LAbs T1 t2 |;| \<sigma>,f\<rparr> |:| R \<Longrightarrow> \<exists>R2. R = T1 \<rightarrow> R2 \<and>  \<Gamma> |,| T1 \<turnstile> \<lparr>t2|;| \<sigma>,f\<rparr> |:| R2 "
+  "\<Gamma> \<turnstile> \<lparr> LApp t1 t2 |;| \<sigma>,f\<rparr> |:| R \<Longrightarrow> \<exists>T11. \<Gamma> \<turnstile> \<lparr>t1|;|\<sigma>,f\<rparr> |:| T11 \<rightarrow> R \<and> \<Gamma> \<turnstile> \<lparr>t2|;| \<sigma>,f\<rparr> |:| T11"
+  "\<Gamma> \<turnstile> \<lparr> unit|;| \<sigma>,f\<rparr> |:| R \<Longrightarrow> R = Unit"
+  "\<Gamma> \<turnstile> \<lparr> Seq t1 t2 |;| \<sigma>,f\<rparr> |:| R \<Longrightarrow> \<exists>A. R = A \<and> \<Gamma> \<turnstile> \<lparr>t2|;| \<sigma>,f\<rparr> |:| A \<and> \<Gamma> \<turnstile> \<lparr>t1|;| \<sigma>,f\<rparr> |:| Unit"
+  "\<Gamma> \<turnstile> \<lparr> t as A |;| \<sigma>,f\<rparr> |:| R \<Longrightarrow> R = A"
+  "\<Gamma> \<turnstile> \<lparr> Let var x := t in t1 |;| \<sigma>,f\<rparr> |:| R \<Longrightarrow> \<exists>A B. R = B \<and> \<Gamma> \<turnstile> \<lparr> t|;| \<sigma>,f\<rparr> |:| A \<and> (insert_nth x A \<Gamma>) \<turnstile> \<lparr>t1|;| \<sigma>,f\<rparr> |:| B"
+  "\<Gamma> \<turnstile> \<lparr> \<lbrace>t1,t2\<rbrace>|;| \<sigma>,f\<rparr> |:| R \<Longrightarrow> \<exists>A B. \<Gamma> \<turnstile> \<lparr> t1|;| \<sigma>,f\<rparr> |:| A \<and> \<Gamma> \<turnstile> \<lparr> t2|;| \<sigma>,f\<rparr> |:| B \<and> R = A |\<times>| B"
+  "\<Gamma> \<turnstile> \<lparr> \<pi>1 t|;| \<sigma>,f1\<rparr> |:| R \<Longrightarrow> \<exists>A B f. f=f1 \<and> \<Gamma> \<turnstile> \<lparr> t|;| \<sigma>,f\<rparr> |:| A |\<times>| B \<and> R = A"
+  "\<Gamma> \<turnstile> \<lparr> \<pi>2 t|;| \<sigma>,f\<rparr> |:| R \<Longrightarrow> \<exists>A B. \<Gamma> \<turnstile> \<lparr> t|;| \<sigma>,f\<rparr> |:| A |\<times>| B \<and> R = B"
+  "\<Gamma> \<turnstile> \<lparr> Tuple L|;| \<sigma>,f\<rparr> |:| R \<Longrightarrow> \<exists>TL. length L = length TL \<and> (\<forall>i. 0\<le>i \<longrightarrow> i< length L \<longrightarrow> \<Gamma> \<turnstile> \<lparr>(L ! i)|;| \<sigma>,f\<rparr> |:| (TL ! i)) \<and> R = \<lparr>TL\<rparr>"
+  "\<Gamma> \<turnstile> \<lparr> (\<Pi> i t)|;| \<sigma>,f\<rparr> |:| R \<Longrightarrow> \<exists>TL. R = (TL ! (i-1)) \<and> \<Gamma> \<turnstile> \<lparr>t|;| \<sigma>,f\<rparr> |:| \<lparr>TL\<rparr> \<and> 1\<le>i \<and> i\<le> length TL"
+  "\<Gamma> \<turnstile> \<lparr> (Record L1 LT)|;| \<sigma>,f\<rparr> |:| R \<Longrightarrow> \<exists>TL. R = \<lparr>L1|:|TL\<rparr> \<and> length TL = length LT \<and> length L1 = length LT \<and> distinct L1 \<and> 
+                                    (\<forall>i. 0\<le>i \<longrightarrow> i< length LT \<longrightarrow> \<Gamma> \<turnstile> \<lparr> (LT ! i)|;| \<sigma>,f\<rparr> |:| (TL ! i)) " 
+  "\<Gamma> \<turnstile> \<lparr> (ProjR l t)|;| \<sigma>,f\<rparr> |:| R \<Longrightarrow>\<exists>m L TL. \<Gamma> \<turnstile> \<lparr>t |;| \<sigma>,f\<rparr> |:| \<lparr>L|:|TL\<rparr> \<and> index L l = m \<and> TL ! m = R \<and> distinct L \<and> length L = length TL
                               \<and> l \<in> set L"
-  "\<Gamma> \<turnstile> \<lparr><|V k as A|>|;|\<sigma>\<rparr> |:| R \<Longrightarrow> \<sigma> k = Some A"
-  "\<Gamma> \<turnstile> \<lparr>Let pattern p := t1 in t2|;|\<sigma>1\<rparr> |:| R \<Longrightarrow>\<exists>\<sigma> B. coherent p B\<and> Lmatch_Type p \<sigma>  \<and> \<Gamma> \<turnstile> \<lparr>t1|;|\<sigma>1\<rparr> |:| B \<and>
-                                                  \<Gamma> \<turnstile> \<lparr>t2|;|(\<sigma> ++  \<sigma>1)\<rparr> |:| R" 
-  "\<Gamma> \<turnstile> \<lparr>inl t as R|;|\<sigma>1\<rparr> |:| R \<Longrightarrow>\<exists>A B. R = A|+|B \<and> \<Gamma> \<turnstile> \<lparr>t|;|\<sigma>1\<rparr> |:| A"
-  "\<Gamma> \<turnstile> \<lparr>inr t as R|;|\<sigma>1\<rparr> |:| R \<Longrightarrow>\<exists>A B. R = A|+|B \<and> \<Gamma> \<turnstile> \<lparr>t|;|\<sigma>1\<rparr> |:| B"
-  "\<Gamma> \<turnstile> \<lparr>Case t of Inl x \<Rightarrow> t1 | Inr y \<Rightarrow> t2|;|\<sigma>1\<rparr> |:| R \<Longrightarrow>\<exists>A B C. R = C \<and> \<Gamma> \<turnstile> \<lparr>t|;|\<sigma>1\<rparr> |:| A|+|B \<and>
-                                                          insert_nth x A \<Gamma> \<turnstile> \<lparr>t1|;|\<sigma>1\<rparr> |:| C \<and> insert_nth y B \<Gamma> \<turnstile> \<lparr>t2|;|\<sigma>1\<rparr> |:| C"
-   "\<Gamma> \<turnstile> \<lparr> <l:=t> as R |;| \<sigma>1 \<rparr> |:| R \<Longrightarrow>\<exists>L TL i. R=<L|,|TL> \<and> \<Gamma> \<turnstile> \<lparr> t |;| \<sigma>1 \<rparr> |:| (TL!i) \<and> l = L!i " 
-    " \<Gamma> \<turnstile> \<lparr> Case t of <L1:=I> \<Rightarrow> LT |;| \<sigma>1\<rparr> |:| A \<Longrightarrow>\<exists>TL. L1\<noteq>\<emptyset> \<and> length I = length L1 \<and> length L1 = length TL \<and> length L1 = length LT \<and>
-      \<Gamma> \<turnstile> \<lparr> t |;| \<sigma>1 \<rparr> |:| <L1|,|TL> \<and> (\<forall>i<length L1. insert_nth (I!i) (TL!i) \<Gamma> \<turnstile> \<lparr>(LT!i)|;| \<sigma>1\<rparr> |:| A)"
+  "\<Gamma> \<turnstile> \<lparr><|V k as A|>|;|\<sigma>,f\<rparr> |:| R \<Longrightarrow>R=A \<and> \<sigma> k = Some A"
+  "\<Gamma> \<turnstile> \<lparr>Let pattern p := t1 in t2|;|\<sigma>1,f\<rparr> |:| R \<Longrightarrow>\<exists>\<sigma> B. coherent p B\<and> Lmatch_Type p \<sigma>  \<and> \<Gamma> \<turnstile> \<lparr>t1|;|\<sigma>1,f\<rparr> |:| B \<and>
+                                                  \<Gamma> \<turnstile> \<lparr>t2|;|(\<sigma> ++  \<sigma>1), f\<rparr> |:| R" 
+  "\<Gamma> \<turnstile> \<lparr>inl t as R1|;|\<sigma>1,f\<rparr> |:| R \<Longrightarrow>R1 = R \<and> (\<exists>A B. R = A|+|B \<and> \<Gamma> \<turnstile> \<lparr>t|;|\<sigma>1,f\<rparr> |:| A)"
+  "\<Gamma> \<turnstile> \<lparr>inr t as R1|;|\<sigma>1,f\<rparr> |:| R \<Longrightarrow>R1 = R \<and> (\<exists>A B. R = A|+|B \<and> \<Gamma> \<turnstile> \<lparr>t|;|\<sigma>1,f\<rparr> |:| B)"
+  "\<Gamma> \<turnstile> \<lparr>Case t of Inl x \<Rightarrow> t1 | Inr y \<Rightarrow> t2|;|\<sigma>1,f\<rparr> |:| R \<Longrightarrow>\<exists>A B C. R = C \<and> \<Gamma> \<turnstile> \<lparr>t|;|\<sigma>1,f\<rparr> |:| A|+|B \<and>
+                                                          insert_nth x A \<Gamma> \<turnstile> \<lparr>t1|;|\<sigma>1,f\<rparr> |:| C \<and> insert_nth y B \<Gamma> \<turnstile> \<lparr>t2|;|\<sigma>1,f\<rparr> |:| C"
+   "\<Gamma> \<turnstile> \<lparr> <l:=t> as R1 |;| \<sigma>1,f \<rparr> |:| R \<Longrightarrow>R=R1 \<and> (\<exists>L TL i. R=<L|,|TL> \<and> \<Gamma> \<turnstile> \<lparr> t |;| \<sigma>1,f \<rparr> |:| (TL!i) \<and> l = L!i \<and> i<length L \<and> length L = length TL)" 
+    " \<Gamma> \<turnstile> \<lparr> Case t of <L1:=I> \<Rightarrow> LT |;| \<sigma>1,f\<rparr> |:| A \<Longrightarrow>\<exists>TL. L1\<noteq>\<emptyset> \<and> length I = length L1 \<and> length L1 = length TL \<and> length L1 = length LT \<and>
+      \<Gamma> \<turnstile> \<lparr> t |;| \<sigma>1,f \<rparr> |:| <L1|,|TL> \<and> (\<forall>i<length L1. insert_nth (I!i) (TL!i) \<Gamma> \<turnstile> \<lparr>(LT!i)|;| \<sigma>1,f\<rparr> |:| A)"
+   "\<Gamma> \<turnstile> \<lparr> fix t |;| \<sigma>,f\<rparr> |:| A \<Longrightarrow> \<Gamma> \<turnstile> \<lparr> t |;| \<sigma>,f\<rparr> |:| A\<rightarrow>A"
+   "\<Gamma> \<turnstile> \<lparr> Lnil A |;| \<sigma>,f\<rparr> |:| R \<Longrightarrow> R = (\<lambda>List A) \<and> f=False"
+   "\<Gamma> \<turnstile> \<lparr> Lhead A t |;| \<sigma>,f\<rparr> |:| R \<Longrightarrow> R = A \<and> \<Gamma> \<turnstile> \<lparr> t |;| \<sigma>, True\<rparr> |:| \<lambda>List A"
+   "\<Gamma> \<turnstile> \<lparr> Lisnil A t |;| \<sigma>,f\<rparr> |:| R \<Longrightarrow> R = Bool \<and> \<Gamma> \<turnstile> \<lparr> t |;| \<sigma>,f\<rparr> |:| \<lambda>List A"
+   "\<Gamma> \<turnstile> \<lparr> Ltail A t |;| \<sigma>,f\<rparr> |:| R \<Longrightarrow> R = (\<lambda>List A) \<and> \<Gamma> \<turnstile> \<lparr> t |;| \<sigma>, True\<rparr> |:| \<lambda>List A"
+   "\<Gamma> \<turnstile> \<lparr> Lcons A t t'|;| \<sigma>,f\<rparr> |:| R \<Longrightarrow> R = (\<lambda>List A) \<and> \<Gamma> \<turnstile> \<lparr> t' |;| \<sigma>,f\<rparr> |:| (\<lambda>List A) \<and> 
+                                        \<Gamma> \<turnstile> \<lparr> t |;| \<sigma>,f\<rparr> |:| A"
 proof -
-  assume H:"\<Gamma> \<turnstile> \<lparr> Let var x := t in t1|;|\<sigma>\<rparr> |:| R"
-  show " \<exists>A B. R = B \<and> \<Gamma> \<turnstile> \<lparr> t|;| \<sigma>\<rparr> |:| A \<and> (insert_nth x A \<Gamma>) \<turnstile> \<lparr>t1|;| \<sigma>\<rparr> |:| B"
+  assume H:"\<Gamma> \<turnstile> \<lparr> Let var x := t in t1|;|\<sigma>,f\<rparr> |:| R"
+  show " \<exists>A B. R = B \<and> \<Gamma> \<turnstile> \<lparr> t|;| \<sigma>,f\<rparr> |:| A \<and> (insert_nth x A \<Gamma>) \<turnstile> \<lparr>t1|;| \<sigma>,f\<rparr> |:| B"
     using has_type_LetE[OF H] 
     by fastforce 
 next
-  assume H1: "\<Gamma> \<turnstile> \<lparr>Let pattern p := t1 in t2|;|\<sigma>1\<rparr> |:| R"
-  show "\<exists>\<sigma> B. coherent p B \<and> Lmatch_Type p \<sigma>  \<and> \<Gamma> \<turnstile> \<lparr>t1|;|\<sigma>1\<rparr> |:| B \<and> \<Gamma> \<turnstile> \<lparr>t2|;|(\<sigma> ++ \<sigma>1)\<rparr> |:| R"
+  assume H1: "\<Gamma> \<turnstile> \<lparr>Let pattern p := t1 in t2|;|\<sigma>1,f\<rparr> |:| R"
+  show "\<exists>\<sigma> B. coherent p B \<and> Lmatch_Type p \<sigma>  \<and> \<Gamma> \<turnstile> \<lparr>t1|;|\<sigma>1,f\<rparr> |:| B \<and> \<Gamma> \<turnstile> \<lparr>t2|;|(\<sigma> ++ \<sigma>1),f\<rparr> |:| R"
     using has_type_LetPE[OF H1]
     by metis
 next
-  assume H2: "\<Gamma> \<turnstile> \<lparr>Case t of Inl x \<Rightarrow> t1 | Inr y \<Rightarrow> t2|;|\<sigma>1\<rparr> |:| R"
-  show "\<exists>A B C. R = C \<and> \<Gamma> \<turnstile> \<lparr>t|;|\<sigma>1\<rparr> |:| A |+| B \<and> insert_nth x A \<Gamma> \<turnstile> \<lparr>t1|;|\<sigma>1\<rparr> |:| C \<and> insert_nth y B \<Gamma> \<turnstile> \<lparr>t2|;|\<sigma>1\<rparr> |:| C"
+  assume H2: "\<Gamma> \<turnstile> \<lparr>Case t of Inl x \<Rightarrow> t1 | Inr y \<Rightarrow> t2|;|\<sigma>1,f\<rparr> |:| R"
+  show "\<exists>A B C. R = C \<and> \<Gamma> \<turnstile> \<lparr>t|;|\<sigma>1,f\<rparr> |:| A |+| B \<and> insert_nth x A \<Gamma> \<turnstile> \<lparr>t1|;|\<sigma>1,f\<rparr> |:| C \<and> insert_nth y B \<Gamma> \<turnstile> \<lparr>t2|;|\<sigma>1,f\<rparr> |:| C"
     using has_type_CaseSE[OF H2]
     by fastforce
 next
-  assume H4: "\<Gamma> \<turnstile> \<lparr><l:=t> as R|;|\<sigma>1\<rparr> |:| R"
-  show  "\<exists>L TL i. R = <L|,|TL> \<and> \<Gamma> \<turnstile> \<lparr>t|;|\<sigma>1\<rparr> |:| (TL ! i) \<and> l = L ! i"
+  assume H4: "\<Gamma> \<turnstile> \<lparr><l:=t> as R1|;|\<sigma>1,f\<rparr> |:| R"
+  show  "R=R1 \<and> (\<exists>L TL i. R = <L|,|TL> \<and> \<Gamma> \<turnstile> \<lparr>t|;|\<sigma>1,f\<rparr> |:| (TL ! i) \<and> l = L ! i \<and> i<length L \<and> length L = length TL)"
     using has_type_VariantE[OF H4]
     by metis    
 next
-  assume H5: "\<Gamma> \<turnstile> \<lparr>Case t of <L1:=I> \<Rightarrow> LT|;|\<sigma>1\<rparr> |:| A"
+  assume H5: "\<Gamma> \<turnstile> \<lparr>Case t of <L1:=I> \<Rightarrow> LT|;|\<sigma>1,f\<rparr> |:| A"
   show "\<exists>TL. L1\<noteq>\<emptyset> \<and> length I = length L1 \<and> length L1 = length TL \<and> length L1 = length LT \<and>
-      \<Gamma> \<turnstile> \<lparr> t |;| \<sigma>1 \<rparr> |:| <L1|,|TL> \<and> (\<forall>i<length L1. insert_nth (I!i) (TL!i) \<Gamma> \<turnstile> \<lparr>(LT!i)|;| \<sigma>1\<rparr> |:| A)"
+      \<Gamma> \<turnstile> \<lparr> t |;| \<sigma>1,f \<rparr> |:| <L1|,|TL> \<and> (\<forall>i<length L1. insert_nth (I!i) (TL!i) \<Gamma> \<turnstile> \<lparr>(LT!i)|;| \<sigma>1,f\<rparr> |:| A)"
     using has_type_CaseVE[OF H5]
     by (metis append_Cons append_Nil insert_nth_take_drop)
-qed (auto elim: has_type_L.cases has_type_ProjTE, metis has_type_ProjRE)
+next
+  assume H: "\<Gamma> \<turnstile> \<lparr> (ProjR l t)|;| \<sigma>,f\<rparr> |:| R"
+  show "\<exists>m L TL. \<Gamma> \<turnstile> \<lparr>t |;| \<sigma>,f\<rparr> |:| \<lparr>L|:|TL\<rparr> \<and> index L l = m \<and> TL ! m = R \<and> distinct L \<and> length L = length TL
+                              \<and> l \<in> set L"
+    using has_type_ProjRE[OF H]
+    by metis
+qed (auto elim: has_type_L.cases has_type_ProjTE)
 
 
 lemma[simp]: "nat (int x + 1) = Suc x" by simp
@@ -338,22 +351,22 @@ qed
 
 lemma weakening :
   fixes \<Gamma>::lcontext  and t::lterm and A S::ltype and \<sigma> ::"nat\<rightharpoonup>ltype" and n::nat
-  assumes well_typed: "\<Gamma> \<turnstile> \<lparr>t|;| \<sigma>\<rparr> |:| A" and
+  assumes well_typed: "\<Gamma> \<turnstile> \<lparr>t|;| \<sigma>,f\<rparr> |:| A" and
           weaker_ctx: " n \<le> length \<Gamma>" 
-  shows "insert_nth n S \<Gamma> \<turnstile> \<lparr>shift_L 1 n t|;| \<sigma>\<rparr> |:| A"
+  shows "insert_nth n S \<Gamma> \<turnstile> \<lparr>shift_L 1 n t|;| \<sigma>,f\<rparr> |:| A"
 using assms 
-proof(induction \<Gamma> t \<sigma> A arbitrary: n rule:has_type_L.induct)
-  case (has_type_LAbs \<Gamma>1 T1 t2 \<sigma>1 T2)
+proof(induction \<Gamma> t \<sigma> f A arbitrary: n rule:has_type_L.induct)
+  case (has_type_LAbs \<Gamma>1 T1 t2 \<sigma>1 f T2)
     
     have "Suc n\<le>length(\<Gamma>1|,|T1)" using has_type_LAbs(3) by auto
 
-    hence "insert_nth (Suc n) S (\<Gamma>1 |,| T1) \<turnstile> \<lparr>shift_L 1 (Suc n) t2|;| \<sigma>1\<rparr> |:| T2"
+    hence "insert_nth (Suc n) S (\<Gamma>1 |,| T1) \<turnstile> \<lparr>shift_L 1 (Suc n) t2|;| \<sigma>1,f\<rparr> |:| T2"
       using has_type_LAbs(2)[where n="Suc n"]
       by auto
     then show ?case
       by (auto intro: has_type_L.has_type_LAbs)              
 next 
-  case(has_type_Tuple L TL \<Gamma>1 \<sigma>1)
+  case(has_type_Tuple L TL \<Gamma>1 \<sigma>1 f)
     show ?case    
       using has_type_Tuple(1,2) nth_map[of _ L "shift_L 1 n"] 
             has_type_Tuple(4)[OF _ _ has_type_Tuple(5)]
@@ -371,9 +384,9 @@ next
             has_type_RCD(6)[OF _ has_type_RCD(7)]           
       by (force intro!: "has_type_L.intros"(16))+
 next
-  case (has_type_Let \<Gamma> t1 \<sigma>1 A x t2 B)
+  case (has_type_Let \<Gamma> t1 \<sigma>1 f A x t2 B)
     
-    have "n \<le> x \<Longrightarrow> (take n \<Gamma> @ drop n \<Gamma> |,| S) \<turnstile> \<lparr>Let var Suc x := shift_L 1 n t1 in shift_L 1 n t2|;| \<sigma>1\<rparr> |:| B"
+    have "n \<le> x \<Longrightarrow> (take n \<Gamma> @ drop n \<Gamma> |,| S) \<turnstile> \<lparr>Let var Suc x := shift_L 1 n t1 in shift_L 1 n t2|;| \<sigma>1,f\<rparr> |:| B"
       using has_type_Let(5) has_type_Let(3)
             has_type_Let(4)[unfolded length_insert_nth,  of n] 
             insert_nth_comp(1)[OF has_type_Let(5), of x S A] 
@@ -392,36 +405,36 @@ next
             hyps(6)[OF hyps(7)]
       by (auto intro: has_type_L.intros(19))
 next
-  case (has_type_Case \<Gamma>1 t \<sigma>1 A B x t1 C y t2)
+  case (has_type_Case \<Gamma>1 t \<sigma>1 f A B x t1 C y t2)
 
 
-    have Sum_type: "insert_nth n S \<Gamma>1 \<turnstile> \<lparr>shift_L 1 n t|;| \<sigma>1\<rparr> |:| A |+| B"
+    have Sum_type: "insert_nth n S \<Gamma>1 \<turnstile> \<lparr>shift_L 1 n t|;| \<sigma>1,f\<rparr> |:| A |+| B"
       using has_type_Case(4)[OF has_type_Case(7)] 
       by auto
 
-    have B1:"n \<le> x \<Longrightarrow> n \<le> y \<Longrightarrow> insert_nth (Suc x) A (insert_nth n S \<Gamma>1) \<turnstile> \<lparr>shift_L 1 n t1|;|\<sigma>1\<rparr> |:| C \<and>
-                                  insert_nth (Suc y) B (insert_nth n S \<Gamma>1) \<turnstile> \<lparr>shift_L 1 n t2|;|\<sigma>1\<rparr> |:| C"
+    have B1:"n \<le> x \<Longrightarrow> n \<le> y \<Longrightarrow> insert_nth (Suc x) A (insert_nth n S \<Gamma>1) \<turnstile> \<lparr>shift_L 1 n t1|;|\<sigma>1,f\<rparr> |:| C \<and>
+                                  insert_nth (Suc y) B (insert_nth n S \<Gamma>1) \<turnstile> \<lparr>shift_L 1 n t2|;|\<sigma>1,f\<rparr> |:| C"
       using  has_type_Case(5)[of n] has_type_Case(7)
              has_type_Case(6)[of n]
              insert_nth_comp(1)[of n \<Gamma>1 _ S _] length_insert_nth
       by (metis le_SucI)+
 
-    have B2: " n \<le> x \<Longrightarrow> \<not> n \<le> y \<Longrightarrow> insert_nth (Suc x) A (insert_nth n S \<Gamma>1) \<turnstile> \<lparr>shift_L 1 n t1|;|\<sigma>1\<rparr> |:| C \<and> 
-                                      insert_nth y B (insert_nth n S \<Gamma>1) \<turnstile> \<lparr>shift_L 1 (Suc n) t2|;|\<sigma>1\<rparr> |:| C"
+    have B2: " n \<le> x \<Longrightarrow> \<not> n \<le> y \<Longrightarrow> insert_nth (Suc x) A (insert_nth n S \<Gamma>1) \<turnstile> \<lparr>shift_L 1 n t1|;|\<sigma>1,f\<rparr> |:| C \<and> 
+                                      insert_nth y B (insert_nth n S \<Gamma>1) \<turnstile> \<lparr>shift_L 1 (Suc n) t2|;|\<sigma>1,f\<rparr> |:| C"
       using  has_type_Case(5)[of n, unfolded length_insert_nth]
              has_type_Case(6)[of "Suc n", unfolded length_insert_nth]  
              has_type_Case(7) insert_nth_comp[of n \<Gamma>1 _ S _] 
       by (metis Suc_le_mono not_le le_SucI)+
 
-    have B3: "\<not> n \<le> x \<Longrightarrow>  n \<le> y \<Longrightarrow> insert_nth x A (insert_nth n S \<Gamma>1) \<turnstile> \<lparr>shift_L 1 (Suc n) t1|;|\<sigma>1\<rparr> |:| C \<and>
-                                      insert_nth (Suc y) B (insert_nth n S \<Gamma>1) \<turnstile> \<lparr>shift_L 1 n t2|;|\<sigma>1\<rparr> |:| C"
+    have B3: "\<not> n \<le> x \<Longrightarrow>  n \<le> y \<Longrightarrow> insert_nth x A (insert_nth n S \<Gamma>1) \<turnstile> \<lparr>shift_L 1 (Suc n) t1|;|\<sigma>1,f\<rparr> |:| C \<and>
+                                      insert_nth (Suc y) B (insert_nth n S \<Gamma>1) \<turnstile> \<lparr>shift_L 1 n t2|;|\<sigma>1,f\<rparr> |:| C"
       using  has_type_Case(5)[of "Suc n", unfolded length_insert_nth]
              has_type_Case(6)[of n, unfolded length_insert_nth]  
              has_type_Case(7) insert_nth_comp[of n \<Gamma>1 _ S _] 
       by (metis Suc_le_mono not_le le_SucI)+
 
-    have B4: "\<not> n \<le> x \<Longrightarrow> \<not> n \<le> y \<Longrightarrow> insert_nth x A (insert_nth n S \<Gamma>1) \<turnstile> \<lparr>shift_L 1 (Suc n) t1|;|\<sigma>1\<rparr> |:| C \<and>
-                                      insert_nth y B (insert_nth n S \<Gamma>1) \<turnstile> \<lparr>shift_L 1 (Suc n) t2|;|\<sigma>1\<rparr> |:| C"
+    have B4: "\<not> n \<le> x \<Longrightarrow> \<not> n \<le> y \<Longrightarrow> insert_nth x A (insert_nth n S \<Gamma>1) \<turnstile> \<lparr>shift_L 1 (Suc n) t1|;|\<sigma>1,f\<rparr> |:| C \<and>
+                                      insert_nth y B (insert_nth n S \<Gamma>1) \<turnstile> \<lparr>shift_L 1 (Suc n) t2|;|\<sigma>1,f\<rparr> |:| C"
        using has_type_Case(5)[of "Suc n", unfolded length_insert_nth]
              has_type_Case(6)[of "Suc n", unfolded length_insert_nth]  
              has_type_Case(7) insert_nth_comp(2)[of n \<Gamma>1 _ S _] 
@@ -432,30 +445,30 @@ next
             has_type_L.intros(22) B1 B2 B3 B4
       by force      
 next
-  case (has_type_CaseV L I TL LT \<Gamma> t \<sigma>1 A)
+  case (has_type_CaseV L I TL LT \<Gamma> t \<sigma>1 f A)
     have branches_wtyped:"\<forall>i<length L.
        insert_nth (map (\<lambda>x. if n \<le> x then nat (int x + 1) else x) I ! i) (TL ! i) (take n \<Gamma> @ drop n \<Gamma> |,| S)
-       \<turnstile> \<lparr>((indexed_map 0 (\<lambda>k. shift_L 1 (if (I!k)<n then Suc n else n)) LT) ! i)|;| \<sigma>1\<rparr> |:| A"
+       \<turnstile> \<lparr>((indexed_map 0 (\<lambda>k. shift_L 1 (if (I!k)<n then Suc n else n)) LT) ! i)|;| \<sigma>1,f\<rparr> |:| A"
       proof (rule+)
         fix i
         assume H:"i<length L"
         have P:"\<And>k. k\<le>length (insert_nth (I ! i) (TL ! i) \<Gamma>) \<Longrightarrow>
-                     insert_nth k S (insert_nth (I ! i) (TL ! i) \<Gamma>) \<turnstile> \<lparr>shift_L 1 k (LT ! i)|;|\<sigma>1\<rparr>|:| A"
+                     insert_nth k S (insert_nth (I ! i) (TL ! i) \<Gamma>) \<turnstile> \<lparr>shift_L 1 k (LT ! i)|;|\<sigma>1,f\<rparr>|:| A"
           using has_type_CaseV(7) H 
           by auto
 
-        then have branches_type_n:"insert_nth n S (insert_nth (I ! i) (TL ! i) \<Gamma>) \<turnstile> \<lparr>shift_L 1 n (LT ! i)|;| \<sigma>1\<rparr> |:| A"
+        then have branches_type_n:"insert_nth n S (insert_nth (I ! i) (TL ! i) \<Gamma>) \<turnstile> \<lparr>shift_L 1 n (LT ! i)|;| \<sigma>1,f\<rparr> |:| A"
           using  has_type_CaseV(8)    
                  length_insert_nth[of "I!i" "TL!i" \<Gamma>]
           by (metis le_SucI)
 
-        have branches_type_Sucn:"insert_nth (Suc n) S (insert_nth (I ! i) (TL ! i) \<Gamma>) \<turnstile> \<lparr>shift_L 1 (Suc n) (LT ! i)|;|\<sigma>1\<rparr> |:| A"
+        have branches_type_Sucn:"insert_nth (Suc n) S (insert_nth (I ! i) (TL ! i) \<Gamma>) \<turnstile> \<lparr>shift_L 1 (Suc n) (LT ! i)|;|\<sigma>1,f\<rparr> |:| A"
           using  has_type_CaseV(8)
                  length_insert_nth[of "I!i" "TL!i" \<Gamma>] P[of "Suc n"]
           by (metis Suc_le_mono)
 
         have 1:"n\<le> I!i \<Longrightarrow> insert_nth (map (\<lambda>x. if n \<le> x then nat (int x + 1) else x) I ! i) (TL ! i) (take n \<Gamma> @ drop n \<Gamma> |,| S)
-                \<turnstile> \<lparr>((indexed_map 0 (\<lambda>k. shift_L 1 (if (I!k)<n then Suc n else n)) LT) ! i)|;|\<sigma>1\<rparr> |:| A"
+                \<turnstile> \<lparr>((indexed_map 0 (\<lambda>k. shift_L 1 (if (I!k)<n then Suc n else n)) LT) ! i)|;|\<sigma>1,f\<rparr> |:| A"
           using has_type_CaseV(1,2,8) H        
           proof -
             
@@ -466,7 +479,7 @@ next
               by (simp add: index_not_index_cong[of 0 "\<lambda>k. shift_L 1 (if I ! k < n then Suc n else n)" LT, simplified])
             
             from branches_type_n
-              have "insert_nth (Suc (I ! i)) (TL ! i) (take n \<Gamma> @ drop n \<Gamma> |,| S) \<turnstile> \<lparr>shift_L 1 n (LT ! i)|;|\<sigma>1\<rparr> |:| A"
+              have "insert_nth (Suc (I ! i)) (TL ! i) (take n \<Gamma> @ drop n \<Gamma> |,| S) \<turnstile> \<lparr>shift_L 1 n (LT ! i)|;|\<sigma>1,f\<rparr> |:| A"
                 using insert_nth_comp(1)[OF hyps(4,1)] H has_type_CaseV(4)
                 by force
             
@@ -475,7 +488,7 @@ next
           qed
 
         have  "\<not> n\<le> I!i \<Longrightarrow> insert_nth (map (\<lambda>x. if n \<le> x then nat (int x + 1) else x) I ! i) (TL ! i) (take n \<Gamma> @ drop n \<Gamma> |,| S)
-                \<turnstile> \<lparr>((indexed_map 0 (\<lambda>k. shift_L 1 (if (I!k)<n then Suc n else n)) LT) ! i)|;|\<sigma>1\<rparr> |:| A"
+                \<turnstile> \<lparr>((indexed_map 0 (\<lambda>k. shift_L 1 (if (I!k)<n then Suc n else n)) LT) ! i)|;|\<sigma>1,f\<rparr> |:| A"
           using has_type_CaseV(1,2,8) H        
           proof -            
             assume hyps:"\<not>n \<le> I ! i" "L \<noteq> \<emptyset>" "length I = length L" "n \<le> length \<Gamma>" "i < length L"
@@ -486,7 +499,7 @@ next
               by (simp add: index_not_index_cong[of 0 "\<lambda>k. shift_L 1 (if I ! k < n then Suc n else n)" LT, simplified])
             
             from branches_type_Sucn
-              have  "insert_nth (I ! i) (TL ! i) (take n \<Gamma> @ drop n \<Gamma> |,| S) \<turnstile> \<lparr>shift_L 1 (Suc n) (LT ! i)|;|\<sigma>1\<rparr> |:| A"
+              have  "insert_nth (I ! i) (TL ! i) (take n \<Gamma> @ drop n \<Gamma> |,| S) \<turnstile> \<lparr>shift_L 1 (Suc n) (LT ! i)|;|\<sigma>1,f\<rparr> |:| A"
                 using insert_nth_comp(2)[OF hyps(4), of "I!i"] hyps(1)[unfolded not_le[of n "I!i"]]
                 by fastforce
 
@@ -495,7 +508,7 @@ next
           qed
 
         with 1 show "insert_nth (map (\<lambda>x. if n \<le> x then nat (int x + 1) else x) I ! i) (TL ! i) (take n \<Gamma> @ drop n \<Gamma> |,| S)
-         \<turnstile> \<lparr>((indexed_map 0 (\<lambda>k. shift_L 1 (if (I!k)<n then Suc n else n)) LT) ! i)|;| \<sigma>1\<rparr> |:| A"
+         \<turnstile> \<lparr>((indexed_map 0 (\<lambda>k. shift_L 1 (if (I!k)<n then Suc n else n)) LT) ! i)|;| \<sigma>1,f\<rparr> |:| A"
           by blast
       qed 
     show ?case
@@ -509,72 +522,225 @@ lemma fill_keep_value:
   "is_value_L v \<Longrightarrow> is_value_L (fill \<sigma> v)"
 by(induction v rule: is_value_L.induct, auto intro: "is_value_L.intros" )
 
+
+lemma Lmatch_Type_det:
+  "Lmatch_Type p \<sigma> \<Longrightarrow> Lmatch_Type p \<sigma>1 \<Longrightarrow> \<sigma> = \<sigma>1"
+by (induction arbitrary: \<sigma>1 rule: Lmatch_Type.induct)
+   (force simp: "Lmatch_Type.simps"[of "V _ as _", simplified],
+     metis (no_types, hide_lams) nth_equalityI 
+            "Lmatch_Type.simps"[of "RCD _ _", simplified])
+
+method inv_type = (match premises in H:"\<Gamma> \<turnstile> \<lparr> t|;| \<sigma>, f\<rparr> |:| A" for \<Gamma> t \<sigma> f A \<Rightarrow>
+                   \<open>simp add:"has_type_L.simps"[of \<Gamma> t \<sigma> f A, simplified]\<close>)  
+    
+theorem uniqueness_of_types:
+  "\<Gamma> \<turnstile> \<lparr>t|;|\<sigma>,f\<rparr> |:| A \<Longrightarrow> \<Gamma> \<turnstile> \<lparr>t|;|\<sigma>,f\<rparr> |:| B \<Longrightarrow> A=B"
+proof (induction \<Gamma> t \<sigma> f A arbitrary:B rule: has_type_L.induct)
+  case (has_type_Tuple L TL \<Gamma> \<sigma> f)
+    note hyps=this
+    show ?case 
+      using inversion(14)[OF hyps(5)]
+            hyps(2,4) List.nth_equalityI[of TL ]
+      by force
+next
+  case (has_type_RCD L LT TL)
+    note hyps=this
+    show ?case 
+      using inversion(16)[OF hyps(7)]
+            hyps(3,4,6)
+            List.nth_equalityI[of TL]
+      by force
+next
+  case (has_type_LetPattern p B1 \<sigma>)
+    note hyps=this
+    show ?case 
+      using inversion(19)[OF hyps(7)]
+            hyps(6) Lmatch_Type_det[OF hyps(2)]
+      by force
+next
+  case (has_type_Case)
+    thus ?case using inversion(22) by blast
+next
+  case (has_type_CaseV)
+    thus ?case using inversion(24) by blast
+next
+  case (has_type_Fix)
+    thus ?case using inversion(25) by blast
+qed (((metis prod.sel ltype.sel inversion(1-13))+)[13],
+     (metis prod.sel ltype.sel inversion(15,17,18,20,21,23,26-30))+)
+
+
+
 lemma canonical_forms:
-  "is_value_L v \<Longrightarrow> \<Gamma> \<turnstile> \<lparr>v|;|\<sigma>\<rparr> |:| Bool \<Longrightarrow> v = LTrue \<or> v = LFalse"
-  "is_value_L v \<Longrightarrow> \<Gamma> \<turnstile> \<lparr>v|;|\<sigma>\<rparr> |:| T1 \<rightarrow> T2 \<Longrightarrow> \<exists>t n. v = LAbs T1 t"
-  "is_value_L v \<Longrightarrow> \<Gamma> \<turnstile> \<lparr>v|;|\<sigma>\<rparr> |:| Unit \<Longrightarrow> v = unit"
-  "is_value_L v \<Longrightarrow> \<Gamma> \<turnstile> \<lparr>v|;|\<sigma>\<rparr> |:| A |\<times>| B \<Longrightarrow> \<exists>v1 v2. is_value_L v1 \<and> is_value_L v2 \<and> v= \<lbrace>v1,v2\<rbrace>"
-  "is_value_L v \<Longrightarrow> \<Gamma> \<turnstile> \<lparr>v|;|\<sigma>\<rparr> |:| \<lparr>TL\<rparr> \<Longrightarrow> \<exists>L. is_value_L (Tuple L) \<and> v = Tuple L \<and> length TL = length L"
-  "is_value_L v \<Longrightarrow> \<Gamma> \<turnstile> \<lparr>v|;|\<sigma>\<rparr> |:| \<lparr>L|:|TL\<rparr> \<Longrightarrow> \<exists>LT. is_value_L (Record L LT) \<and> v = (Record L LT)" 
-  "is_value_L v \<Longrightarrow> \<Gamma> \<turnstile> \<lparr>v|;|\<sigma>\<rparr> |:| A|+|B \<Longrightarrow> (\<exists>v1. is_value_L v1 \<and> v = inl v1 as A|+|B) \<or> (\<exists>v1. v = inr v1 as A|+|B \<and> is_value_L v1)"
-  "is_value_L v \<Longrightarrow> \<Gamma> \<turnstile> \<lparr>v|;|\<sigma>\<rparr> |:| \<lambda>List A \<Longrightarrow> (v = Lnil A) \<or> (\<exists>v1 v2. is_value_L v1 \<and> is_value_L v2 \<and>
-                                                                v = Lcons A v1 v2)"
+  "is_value_L v \<Longrightarrow> \<Gamma> \<turnstile> \<lparr>v|;|\<sigma>,f\<rparr> |:| Bool \<Longrightarrow> v = LTrue \<or> v = LFalse"
+  "is_value_L v \<Longrightarrow> \<Gamma> \<turnstile> \<lparr>v|;|\<sigma>,f\<rparr> |:| T1 \<rightarrow> T2 \<Longrightarrow> \<exists>t n. v = LAbs T1 t"
+  "is_value_L v \<Longrightarrow> \<Gamma> \<turnstile> \<lparr>v|;|\<sigma>,f\<rparr> |:| Unit \<Longrightarrow> v = unit"
+  "is_value_L v \<Longrightarrow> \<Gamma> \<turnstile> \<lparr>v|;|\<sigma>,f\<rparr> |:| A |\<times>| B \<Longrightarrow> (\<exists>v1 v2. is_value_L v1 \<and> is_value_L v2 \<and> v= \<lbrace>v1,v2\<rbrace>)"
+  "is_value_L v \<Longrightarrow> \<Gamma> \<turnstile> \<lparr>v|;|\<sigma>,f\<rparr> |:| \<lparr>TL\<rparr> \<Longrightarrow> (\<exists>L. is_value_L (Tuple L) \<and> v = Tuple L \<and> length TL = length L)"
+  "is_value_L v \<Longrightarrow> \<Gamma> \<turnstile> \<lparr>v|;|\<sigma>,f\<rparr> |:| \<lparr>L|:|TL\<rparr> \<Longrightarrow> (\<exists>LT. is_value_L (Record L LT) \<and> v = (Record L LT))" 
+  "is_value_L v \<Longrightarrow> \<Gamma> \<turnstile> \<lparr>v|;|\<sigma>,f\<rparr> |:| <L|,|TL> \<Longrightarrow> (\<exists>i v1. i<length L \<and> is_value_L v1 \<and> v = <(L!i):=v1> as <L|,|TL>)"
+  "is_value_L v \<Longrightarrow> \<Gamma> \<turnstile> \<lparr>v|;|\<sigma>,f\<rparr> |:| A|+|B \<Longrightarrow> (\<exists>v1. is_value_L v1 \<and> v = inl v1 as A|+|B) \<or> (\<exists>v1. v = inr v1 as A|+|B \<and> is_value_L v1)"
+  "is_value_L v \<Longrightarrow> \<Gamma> \<turnstile> \<lparr>v|;|\<sigma>,f\<rparr> |:| \<lambda>List A \<Longrightarrow> (v = Lnil A \<and> f=False) \<or> (\<exists>v1 v2. is_value_L v1 \<and> is_value_L v2 \<and> v = Lcons A v1 v2)"
 proof -
   assume  val: "is_value_L v" and 
-          typed: "\<Gamma> \<turnstile> \<lparr>v|;|\<sigma>\<rparr> |:| A|+|B"
+          typed: "\<Gamma> \<turnstile> \<lparr>v|;|\<sigma>,f\<rparr> |:| A|+|B"
   show "(\<exists>v1. is_value_L v1 \<and> v = inl v1 as A|+|B) \<or> (\<exists>v1. v = inr v1 as A|+|B \<and> is_value_L v1)"
+    using val typed
+    by (induction rule: is_value_L.induct, auto elim: "has_type_L.cases")           
+next
+   assume  val: "is_value_L v" and 
+          typed: "\<Gamma> \<turnstile> \<lparr>v|;|\<sigma>,f\<rparr> |:| <L|,|TL>"
+  show "\<exists>i v1. i<length L \<and> is_value_L v1 \<and> v = <(L!i):=v1> as <L|,|TL>"
     using val typed
     by (induction rule: is_value_L.induct, auto elim: "has_type_L.cases")
 qed (auto elim: "is_value_L.cases" "has_type_L.cases")  
 
+
+
+
+lemma coherent_val_imp_Lmatch:
+  "coherent p A \<Longrightarrow> \<Gamma>\<turnstile> \<lparr>t|;|\<sigma>,f\<rparr> |:| A \<Longrightarrow> is_value_L t \<Longrightarrow>\<exists>\<sigma>. Lmatch p t \<sigma>"
+proof (induction arbitrary:t \<Gamma> \<sigma> f rule:coherent.induct)
+  case (2 L PL TL)
+    note hyps=this
+    obtain LT where H:"is_value_L (Record L LT)" "t = Record L LT"
+      using canonical_forms(6)[OF hyps(7,6)]
+      by blast
+         
+    note lenTL_LT = hyps(6)[unfolded H(2) has_type_L.simps[of _ "Record L LT" _ _ "\<lparr>L|:|TL\<rparr>", simplified],
+                        THEN conjunct2, THEN conjunct2, THEN conjunct1]
+         and TL_types = hyps(6)[unfolded H(2) has_type_L.simps[of _ "Record L LT" _ _ "\<lparr>L|:|TL\<rparr>", simplified],
+                        THEN conjunct2, THEN conjunct2, THEN conjunct2, THEN conjunct2]
+      
+    have exF:"\<exists>F. (\<forall>i<length PL. Lmatch (PL ! i) (LT ! i) (F!i)) \<and> length F = length PL"
+      using lenTL_LT TL_types H(1)[unfolded is_value_L.simps[of "Record L LT", simplified]]
+            hyps(3)[symmetric] hyps(5)[of _ \<Gamma> "LT!_" \<sigma> f]
+      proof (induction PL arbitrary: TL LT)
+        case (Cons p PL')
+          obtain l LT' Ta TL' where l_decomp:"TL = Ta # TL'" "LT= l#LT'" "length TL'= length PL'"
+                                             "length LT' = length PL'"
+            using Cons(2,5) length_Suc_conv by metis
+          show ?case
+            using Cons(1)[OF _ _ _ l_decomp(3),of LT'] l_decomp(3,4)
+                  Cons(3,4,6)[unfolded l_decomp(1,2)]
+                 
+            sorry
+      qed simp
+    have "\<And>i. i < length PL \<Longrightarrow> Lmatch (PL ! i) (LT ! i) (F ! i)"
+      proof -
+        fix i 
+        assume inf_len: "i<length PL"
+        obtain \<sigma> where "Lmatch (PL ! i) (LT ! i) \<sigma>"
+          using exF(2) H(1)[unfolded is_value_L.simps[of "Record L LT", simplified]]
+                hyps(6)[unfolded H(2) has_type_L.simps[of _ "Record L LT" _ _ "\<lparr>L|:|TL\<rparr>", simplified],
+                        THEN conjunct2, THEN conjunct2]
+                hyps(3)[symmetric] hyps(5)[of i \<Gamma> "LT!i" \<sigma> f] inf_len
+          by presburger
+        then show "Lmatch (PL ! i) (LT ! i) (F ! i)"
+          using exF(1) inf_len 
+          by presburger
+      qed          
+       
+    then show ?case
+      using "Lmatch.intros"(2)[OF _ _ exF(2) _ H(1)]
+            hyps(6)[unfolded H(2) has_type_L.simps[of _ "Record L LT" _ _ "\<lparr>L|:|TL\<rparr>", simplified]]
+            hyps(3) H(2)
+      by force
+qed (auto intro: Lmatch.intros) 
+
 lemma progress:
-  "\<emptyset> \<turnstile> \<lparr>t|;|empty\<rparr> |:| A \<Longrightarrow> is_value_L t \<or> (\<exists>t1. eval1_L t t1)"
-proof (induction "\<emptyset>::ltype list" t "empty::nat\<rightharpoonup>ltype" A rule: has_type_L.induct)
+  "\<emptyset> \<turnstile> \<lparr>t|;|empty, f\<rparr> |:| A \<Longrightarrow> is_value_L t \<or> (\<exists>t1. eval1_L t t1)"
+proof (induction "\<emptyset>::ltype list" t "empty::nat\<rightharpoonup>ltype" f A rule: has_type_L.induct)
   case (has_type_LIf t1 t2 A t3)
     thus ?case by (metis eval1_L.intros canonical_forms)
-next
-  case (has_type_LetPattern)
-    thus ?case sorry
 next
   case (has_type_Tuple L TL)
     note hyps=this
     have "(\<exists>j<length L. (\<forall>i<j. is_value_L (L ! i)) \<and> (\<exists>t1. eval1_L (L ! j) t1))\<or>
           is_value_L (Tuple L)"
-      
-      sorry
-    thus ?case sorry
+      using hyps(4)
+      proof (induction L)
+        case Nil
+          show ?case 
+            using "is_value_L.intros"(6)[of \<emptyset>, simplified]
+            by blast
+      next
+        case (Cons a L')
+          have "is_value_L a\<Longrightarrow> ?case"
+            using Cons(1)[OF Cons(2)[of "Suc _", simplified], simplified] "is_value_L.intros"(6)[of "a#L'"]
+                  "is_value_L.simps"[of "Tuple _", simplified]
+            by meson (metis Suc_less_eq nth_Cons_0 nth_Cons_Suc old.nat.exhaust length_Cons,
+                   metis One_nat_def Suc_pred le_imp_less_Suc length_Cons less_SucE not_less_eq nth_Cons')
+          then show ?case
+            using Cons(2)[of 0, simplified]
+            by fastforce
+      qed 
+    then show ?case
+      using eval1_L_Tuple[of "Suc _" L, simplified] "is_value_L.intros"(6)[of "take _ L", simplified]
+      by force
 next
-  case (has_type_RCD)
-    thus ?case sorry
+  case (has_type_RCD L LT TL)
+    note hyps=this
+    have "(\<exists>j<length LT. (\<forall>i<j. is_value_L (LT ! i)) \<and> (\<exists>t1. eval1_L (LT ! j) t1))\<or>
+          is_value_L (Record L LT)"
+      using hyps(2-4,6)
+      proof (induction LT arbitrary: L TL)
+        case Nil
+          show ?case 
+            using "is_value_L.intros"(7)[of \<emptyset>, simplified]
+            by blast
+      next
+        case (Cons a LT')
+          obtain l L' t TL' where l_prop:"L = l#L'" "length L' = length LT'"
+                                  "TL = t#TL'" "length LT' = length TL'"
+            using length_Suc_conv Cons(3,4)
+            by metis
+
+          note dist_L' = Cons(2)[unfolded l_prop(1) distinct.simps(2)[of l L'], THEN conjunct2]
+
+          have "is_value_L a\<Longrightarrow> ?case"
+            using Cons(1)[OF dist_L' l_prop(4,2) Cons(5)[of "Suc _", simplified], simplified] 
+            by meson (metis Suc_less_eq nth_Cons_0 nth_Cons_Suc old.nat.exhaust length_Cons,
+                      metis One_nat_def Suc_less_eq Suc_pred le_neq_implies_less length_Cons nth_Cons'
+                            "is_value_L.intros"(7) "is_value_L.simps"[of "Record L' LT'", simplified])              
+          then show ?case
+            using Cons(5)[of 0, simplified]
+            by fastforce
+      qed 
+    then show ?case
+      using eval1_L_RCD[of _ LT L] "is_value_L.intros"(7)[of "take _ LT" "take _ L", simplified]
+      by force
 next
   case (has_type_ProjT i TL t)
    thus ?case 
      by (metis eval1_L.intros canonical_forms)     
 next
-  case (has_type_CaseV L I TL LT t A)
+  case (has_type_CaseV L I TL LT t f A)
     note hyps=this
     show ?case
-      sorry
+      using eval1_L.intros(32,33) hyps(6) canonical_forms(7)[OF _ hyps(5)]
+      by metis
 next
-  case (has_type_head t A)
+  case (has_type_Case t f A B x t1 C y t2)
     note hyps=this
     show ?case
       using canonical_forms(8)[OF _ hyps(1)]
-            hyps(2)
+            hyps(2) eval1_L.intros(27-29)
+      by blast
+next
+  case (has_type_LetPattern p B \<sigma> t1 f t2 A)
+    note hyps=this
+    have 1:"\<exists>n A. p = V n as A \<and> B = A \<Longrightarrow> is_value_L t1 \<Longrightarrow> ?case"
+      using "Lmatch.intros"(1) eval1_L.intros(25) 
+      by fast
+    have "(\<exists>L PL TL. p = RCD L PL \<and> B = \<lparr>L|:|TL\<rparr> \<and> distinct L \<and> distinct (Pvars (RCD L PL)) \<and> length L = length PL 
+            \<and> length PL = length TL \<and> (\<forall>x<length TL. coherent (PL ! x) (TL ! x))) \<Longrightarrow> ?case"
+      using "Lmatch.intros"(2) eval1_L.intros(25)
       sorry
-next
-  case (has_type_tail t A)
-     note hyps=this
-    show ?case
-      using canonical_forms(8)[OF _ hyps(1)]
-            hyps(2)
-      sorry
-next
-  case (has_type_Variant t TL i)
-    thus ?case sorry
-next
-  case (has_type_isNil)
-    thus ?case sorry
+    with 1 show ?case 
+      using hyps(4) hyps(1)[unfolded "coherent.simps"[of p]]
+            eval1_L.intros(26) 
+      by fast
 qed (force intro!: is_value_L.intros eval1_L.intros dest: canonical_forms)+
 
 end
